subnodes. starting isValid proof

verif/btrees_sep.v
@@ -95,6 +95,32 @@ Qed.
 
 Hint Resolve btnode_valid_pointer: valid_pointer.
 
+Lemma btnode_rep_getval: forall n pn,
+    btnode_rep n pn = !!(pn = getval n) && btnode_rep n pn.
+Proof.
+  intros. apply pred_ext; unfold btnode_rep; entailer!.
+Qed.
+
+Lemma unfold_btnode_rep: forall n p,
+    btnode_rep n p =
+  match n with btnode ptr0 le b First Last x =>
+  !!(x=p) &&
+  malloc_token Tsh tbtnode p *
+  field_at Tsh tbtnode (DOT _numKeys) (Vint(Int.repr (Z.of_nat (numKeys n)))) p *
+  field_at Tsh tbtnode (DOT _isLeaf) (Val.of_bool b) p *
+  field_at Tsh tbtnode (DOT _FirstLeaf) (Val.of_bool First) p *
+  field_at Tsh tbtnode (DOT _LastLeaf) (Val.of_bool Last) p *
+  match ptr0 with
+  | None => field_at Tsh tbtnode (DOT _ptr0) nullval p
+  | Some n' => match n' with btnode _ _ _ _ _ p' => field_at Tsh tbtnode (DOT _ptr0) p' p * btnode_rep n' p' end
+  end *
+  field_at Tsh tbtnode (DOT _entries) (le_to_list_complete le) p *
+  le_iter_sepcon le
+  end.
+Proof.
+  intros. destruct n as [ptr0 le b First Last x]. apply pred_ext; simpl; entailer!.
+Qed.
+
 Definition relation_rep (r:relation val) (p:val):mpred :=
   match r with
   | (n,c,d,x) => !!(x=p) &&
@@ -170,62 +196,70 @@ Proof.
 Qed.    
 
 Hint Resolve cursor_rep_valid_pointer: valid_pointer.
-  
+
+Inductive subchild {X:Type} : node X -> listentry X -> Prop :=
+| sc_eq: forall k n le, subchild n (cons X (keychild X k n) le)
+| sc_cons: forall e n le, subchild n le -> subchild n (cons X e le).
+
 Inductive subnode {X:Type} : node X -> node X -> Prop :=
 | sub_refl: forall n, subnode n n
 | sub_ptr0: forall n le b First Last x, subnode n (btnode X (Some n) le b First Last x)
-| sub_entr: forall n p le b First Last x k, subnode n (btnode X p (cons X (keychild X k n) le) b First Last x)
-| sub_cons: forall n p le e b First Last x, subnode n (btnode X p le b First Last x) ->
-                                 subnode n (btnode X p (cons X e le) b First Last x)
+| sub_child: forall n le ptr0 b First Last x, subchild n le -> subnode n (btnode X ptr0 le b First Last x)
 | sub_trans: forall n n1 n2, subnode n n1 -> subnode n1 n2 -> subnode n n2.
 
+Lemma btnode_rep_simpl_ptr0: forall le b x (p0:option (node val)) le0 b0 x0 proot p0 First Last F L,
+    btnode_rep (btnode val (Some (btnode val p0 le0 b0 F L x0)) le b First Last x) proot =
+    !!(x=proot) &&
+      malloc_token Tsh tbtnode proot *
+    field_at Tsh tbtnode (DOT _numKeys) (Vint(Int.repr (Z.of_nat (numKeys_le le)))) proot *
+    field_at Tsh tbtnode (DOT _isLeaf) (Val.of_bool b) proot *
+    field_at Tsh tbtnode (DOT _ptr0) x0 proot *
+    field_at Tsh tbtnode (DOT _FirstLeaf) (Val.of_bool First) proot *
+    field_at Tsh tbtnode (DOT _LastLeaf) (Val.of_bool Last) proot *
+    btnode_rep (btnode val p0 le0 b0 F L x0) x0 *
+    field_at Tsh tbtnode (DOT _entries) (le_to_list_complete le) proot *
+    le_iter_sepcon le.
+Proof.
+  intros. apply pred_ext; entailer!; simpl; entailer!.
+Qed.
 
-(* Lemma btnode_rep_simpl_ptr0: forall le b x (p0:option (node val)) le0 b0 x0 proot p0 First Last, *)
-(*     btnode_rep (btnode val (Some (btnode val p0 le0 b0 x0)) le b First Last x) proot = *)
-(*     !!(x=proot) && *)
-(*       malloc_token Tsh tbtnode proot * *)
-(*     field_at Tsh tbtnode (DOT _numKeys) (Vint(Int.repr (Z.of_nat (numKeys_le le)))) proot * *)
-(*     field_at Tsh tbtnode (DOT _isLeaf) (Val.of_bool b) proot * *)
-(*     field_at Tsh tbtnode (DOT _ptr0) x0 proot * *)
-(*     btnode_rep (btnode val p0 le0 b0 x0) x0 * *)
-(*     field_at Tsh tbtnode (DOT _entries) (le_to_list_complete le) proot * *)
-(*     le_iter_sepcon le. *)
-(* Proof. *)
-(*   intros. apply pred_ext; entailer!; simpl; entailer!. *)
-(* Qed. *)
-
-(* Lemma btnode_rep_simpl_keychild: forall ptr0 le b x proot k nptr0 nle nb nx, *)
-(*     btnode_rep (btnode val ptr0 (cons val (keychild val k (btnode val nptr0 nle nb nx)) le) b x) proot = *)
-(*     !!(x=proot) && *)
-(*       malloc_token Tsh tbtnode proot * *)
-(*     field_at Tsh tbtnode (DOT _numKeys) (Vint(Int.repr (Z.of_nat (S (numKeys_le le))))) proot * *)
-(*     field_at Tsh tbtnode (DOT _isLeaf) (Val.of_bool b) proot * *)
-(*     match ptr0 with *)
-(*     | None => field_at Tsh tbtnode (DOT _ptr0) nullval proot *)
-(*     | Some n' => match n' with btnode _ _ _ p' => field_at Tsh tbtnode (DOT _ptr0) p' proot * btnode_rep n' p' end *)
-(*     end * *)
-(*     field_at Tsh tbtnode (DOT _entries) (le_to_list_complete (cons val (keychild val k (btnode val nptr0 nle nb nx)) le)) proot * *)
-(*     btnode_rep (btnode val nptr0 nle nb nx) nx * *)
-(*     le_iter_sepcon le. *)
-(* Proof. *)
-(*   intros. apply pred_ext; entailer!; simpl; entailer!. *)
-(* Qed. *)
+Theorem subchild_rep: forall n le,
+    subchild n le ->
+    le_iter_sepcon le |-- EX pn:val, btnode_rep n pn * (btnode_rep n pn -* le_iter_sepcon le).
+Proof.
+  intros.
+  induction le. inv H.
+  inversion H.
+  - simpl. destruct n as [ptr0 nle isLeaf First Last x].
+    Exists x. cancel. rewrite <- wand_sepcon_adjoint. cancel.
+  - apply IHle in H2. simpl. eapply derives_trans.
+    apply cancel_left. apply H2. Intros pn. Exists pn. cancel.
+    rewrite <- wand_sepcon_adjoint. cancel. rewrite sepcon_comm.
+    apply wand_frame_elim.
+Qed.
 
 Theorem subnode_rep: forall n root proot,
     subnode n root ->
-    btnode_rep root proot |-- EX pn:val, btnode_rep n pn *
+    btnode_rep root proot = EX pn:val, btnode_rep n pn * (* pn is getval of n *)
                               (btnode_rep n pn -* btnode_rep root proot).
 Proof.
-  (* intros. *)
-  (* induction H. *)
-  (* - Exists proot. cancel. rewrite <- wand_sepcon_adjoint. cancel. *)
-  (* - destruct n. Exists v. rewrite btnode_rep_simpl_ptr0 by auto. *)
-  (*   entailer!. rewrite <- wand_sepcon_adjoint. entailer!. *)
-  (* - destruct n. Exists v. rewrite btnode_rep_simpl_keychild. *)
-  (*   entailer!. rewrite <- wand_sepcon_adjoint. entailer!. *)
-  (* - admit.                      (* we can't use the induction hypothesis *) *)
-  (* - admit.                      (* same *) *)
-Admitted.
+  intros. apply pred_ext.
+  generalize dependent proot.
+  induction H; intros.
+  - Exists proot. cancel. rewrite <- wand_sepcon_adjoint. cancel.
+  - destruct n. Exists v. rewrite btnode_rep_simpl_ptr0 by auto.
+    entailer!. rewrite <- wand_sepcon_adjoint. entailer!.
+  - apply subchild_rep in H.
+    simpl. eapply derives_trans. apply cancel_left. apply H.
+    Intros pn. Exists pn. cancel. rewrite <- wand_sepcon_adjoint.
+    autorewrite with norm. cancel. rewrite wand_sepcon_adjoint. cancel.
+  - eapply derives_trans. apply IHsubnode2.
+    Intros p1. rewrite sepcon_comm.
+    eapply derives_trans. apply cancel_left.
+    apply IHsubnode1. normalize. Exists pn. entailer!. rewrite sepcon_comm.
+    apply wand_frame_ver.
+  - Intros pn. apply wand_frame_elim.
+Qed.
 
 Fixpoint cursor_correct {X:Type} (c:cursor X) (n:node X) (root:node X): Prop :=
   match c with
@@ -236,13 +270,17 @@ Fixpoint cursor_correct {X:Type} (c:cursor X) (n:node X) (root:node X): Prop :=
 Definition get_root {X:Type} (rel:relation X) : node X := fst(fst (fst rel)).
 
 Definition cursor_correct_rel {X:Type} (c:cursor X) (rel:relation X): Prop :=
-  match c with
-  | [] => True
-  | (n,i)::c' => match nth_node i n with
-                 | None => False
-                 | Some n' => cursor_correct c n' (get_root rel)
-                 end
-  end.
+  cursor_correct c (currNode c rel) (get_root rel).
+
+Lemma nth_le_subchild: forall X i (n:node X) le,
+    nth_node_le i le = Some n -> subchild n le.
+Proof.
+  intros. generalize dependent le. induction i.
+  - intros. simpl in H. destruct le; try inv H. destruct e; try inv H1.
+    apply sc_eq.
+  - intros. simpl in H. destruct le; try inv H. apply IHi in H1.
+    apply sc_cons. auto.
+Qed.
 
 Lemma nth_subnode: forall X i (n:node X) n',
     nth_node i n' = Some n -> subnode n n'.
@@ -253,9 +291,10 @@ Proof.
   - destruct n' as [ptr0 le isLeaf x]. simpl in H.
     generalize dependent n. generalize dependent le. induction n0.
     + intros. destruct le; simpl in H. inv H. destruct e; inv H.
-      apply sub_entr.
+      apply sub_child. apply sc_eq.
     + intros. simpl in H. destruct le. inv H.
-      apply IHn0 in H. apply sub_cons. auto.
+      apply nth_le_subchild in H.
+      apply sub_child. apply sc_cons. auto.
 Qed.
 
 Theorem cursor_subnode: forall X (c:cursor X) root n,
