verif/verif_isvalid.v
@@ -22,20 +22,67 @@ Proof.
   start_function.
   forward_call(r,pr,c,pc).      (* t'1=entryIndex(cursor) *)
   forward_call(r,pr,c,pc).      (* t'2=currNode *)
-  (* forward.                      (* t'5=t'2->numKeys *) *)
+  unfold cursor_correct_rel in H0.
+  apply cursor_subnode in H0.
+  unfold relation_rep.
+  destruct r as [[[root numRec] depth] prel]. autorewrite with norm.
+  pose (r:=(root,numRec,depth,prel)).
+  Intros proot. rewrite subnode_rep with (n:=currNode c (root,numRec,depth,prel)) by auto.
+  Intros pcurr. subst. rewrite btnode_rep_getval at 1. normalize.
+  pose (pcurr:=(getval (currNode c (root, numRec, depth, pr)))).
+  rewrite unfold_btnode_rep at 1. fold pcurr.
+  destruct (currNode c (root,numRec,depth,pr)) as [ptr0 le b First Last x]. Intros.
+  pose (currnode:= btnode val ptr0 le b First Last x).
+  forward.                      (* t'5=t'2->numKeys *)
+  simpl in pcurr.
+
+  forward_if (
+     (PROP ( )
+     LOCAL (temp _t'5 (Vint (Int.repr (Z.of_nat (numKeys (btnode val ptr0 le b First Last x)))));
+            temp _t'2 pcurr; temp _t'1 (rep_index (entryIndex c)); temp _cursor pc;
+            temp _t'3 (Val.of_bool (isValid c)) (* new local *)
+           )
+     SEP (field_at Tsh trelation [StructField _root] proot pr; malloc_token Tsh tbtnode pcurr;
+     field_at Tsh tbtnode [StructField _numKeys]
+       (Vint (Int.repr (Z.of_nat (numKeys (btnode val ptr0 le b First Last x))))) pcurr;
+     field_at Tsh tbtnode [StructField _isLeaf] (Val.of_bool b) pcurr;
+     field_at Tsh tbtnode [StructField _FirstLeaf] (Val.of_bool First) pcurr;
+     field_at Tsh tbtnode [StructField _LastLeaf] (Val.of_bool Last) pcurr;
+     match ptr0 with
+     | Some (@btnode _ _ _ _ _ _ p' as n') =>
+         field_at Tsh tbtnode [StructField _ptr0] p' pcurr * btnode_rep n' p'
+     | None => field_at Tsh tbtnode [StructField _ptr0] nullval pcurr
+     end; field_at Tsh tbtnode [StructField _entries] (le_to_list_complete le) pcurr;
+     le_iter_sepcon le; btnode_rep (btnode val ptr0 le b First Last x) pcurr -* btnode_rep root proot;
+     field_at Tsh trelation [StructField _numRecords] (Vint (Int.repr (Z.of_nat numRec))) pr;
+     field_at Tsh trelation [StructField _depth] (Vint (Int.repr (Z.of_nat depth))) pr;
+     malloc_token Tsh trelation pr; cursor_rep c (root, numRec, depth, pr) pc; emp)))%assert.
+
+  - forward_call(r,pr,c,pc).
+    + admit.
+    + admit.
+  - forward.                    (* t'3=0 *)
+    admit.
+  - admit.
 Admitted.
-
-
   
 Lemma body_RL_CursorIsValid: semax_body Vprog Gprog f_RL_CursorIsValid RL_CursorIsValid_spec.
 Proof.
   start_function.
-  (* need to prove entryIndex and currNode first *)
-Admitted.
+  forward_if (
+      (PROP (pc<>nullval)  LOCAL (temp _cursor pc)  SEP (relation_rep r pr; cursor_rep c r pc))).
+  - forward. entailer!.
+  - subst. assert_PROP(False).
+    entailer!. inv H1.
+  - forward_call(r,pr,c,pc).
+    Intros vret. forward.
+    entailer!. unfold force_val, sem_cast_pointer.
+    destruct (isValid c); simpl; auto.
+Qed.
 
 Lemma body_isFirst: semax_body Vprog Gprog f_isFirst isFirst_spec.
 Proof.
   start_function.
-  (* need to prove entryIndex and currNode first *)
+  (* proof should be similar to isvalid *)
 Admitted.
  
